Almost done with the core of HigherOrderContracts

state/HigherOrderContracts.fst
@@ -8,7 +8,21 @@ open SharedRefs
 open Witnessable
 open TargetLang
 
-type resexn a = either a unit
+type err =
+| Contract_failure : string -> err
+
+instance witnessable_err : witnessable err = {
+  satisfy = (fun _ _ -> True);
+  satisfy_on_heap = (fun _ _ _ -> True);
+  satisfy_on_heap_monotonic = (fun _ _ _ _ -> ());
+  pwitness = (fun _ _ -> (fun () -> ()));
+}
+
+instance targetlang_err : targetlang default_spec err = {
+  wt = witnessable_err
+}
+
+type resexn a = either a err
 
 class exportable_from (styp: Type u#a) = {
   [@@@no_method] c_styp : witnessable styp;
@@ -19,9 +33,11 @@ class exportable_from (styp: Type u#a) = {
 }
 
 class safe_importable_to (styp: Type u#a) = {
+  [@@@no_method] c_styp : witnessable styp;
   [@@@no_method] ityp : Type u#b;
   [@@@no_method] c_ityp : targetlang default_spec ityp;
-  [@@@no_method] import : ityp -> styp;
+  [@@@no_method] safe_import : ityp -> styp;
+  [@@@no_method] lemma_safe_import_preserves_prref : x:ityp -> Lemma (requires (c_ityp.wt.satisfy x (Mktuple3?._2 default_spec))) (ensures (c_styp.satisfy (safe_import x) (Mktuple3?._2 default_spec)))
 }
 
 class importable_to (styp: Type u#a) = {
@@ -29,6 +45,7 @@ class importable_to (styp: Type u#a) = {
   [@@@no_method] ityp : Type u#b;
   [@@@no_method] c_ityp : targetlang default_spec ityp;
   [@@@no_method] import : ityp -> resexn styp;
+  [@@@no_method] lemma_import_preserves_prref : x:ityp -> Lemma (requires (c_ityp.wt.satisfy x (Mktuple3?._2 default_spec))) (ensures ((witnessable_sum styp err).satisfy (import x) (Mktuple3?._2 default_spec)))
 }
 
 (** Exportable instances **)
@@ -39,8 +56,54 @@ instance targetlang_is_exportable t {| c1:targetlang default_spec t |} : exporta
   export = (fun x -> x);
   lemma_export_preserves_prref = (fun _ -> ()) }
 
-instance exportable_unit : exportable_from unit = admit ()
-instance exportable_sum t1 t2 {| c1:exportable_from t1 |} {| c2:exportable_from t2 |} : exportable_from (either t1 t2) = admit ()
+instance exportable_unit : exportable_from unit = {
+  c_styp = witnessable_unit;
+  ityp = unit;
+  c_ityp = solve;
+  export = (fun x -> x);
+  lemma_export_preserves_prref = (fun _ -> ())
+}
+
+instance exportable_err : exportable_from err = {
+  c_styp = witnessable_err;
+  ityp = err;
+  c_ityp = solve;
+  export = (fun x -> x);
+  lemma_export_preserves_prref = (fun _ -> ())
+}
+
+instance exportable_int : exportable_from int = {
+  c_styp = witnessable_int;
+  ityp = int;
+  c_ityp = solve;
+  export = (fun x -> x);
+  lemma_export_preserves_prref = (fun _ -> ())
+}
+
+instance exportable_option t {| c:exportable_from t |} : exportable_from (option t) = {
+  c_styp = witnessable_option t #c.c_styp;
+  ityp = option c.ityp;
+  c_ityp = targetlang_option default_spec c.ityp #c.c_ityp;
+  export = (fun x -> match x with | Some x -> Some (c.export x) | FStar.Pervasives.Native.None -> FStar.Pervasives.Native.None);
+  lemma_export_preserves_prref = (fun x -> match x with | Some x -> c.lemma_export_preserves_prref x | FStar.Pervasives.Native.None -> ())
+}
+
+instance exportable_sum t1 t2 {| c1:exportable_from t1 |} {| c2:exportable_from t2 |} : exportable_from (either t1 t2) = {
+  c_styp = witnessable_sum t1 t2 #c1.c_styp #c2.c_styp;
+  ityp = either c1.ityp c2.ityp;
+  c_ityp = targetlang_sum default_spec _ _ #c1.c_ityp #c2.c_ityp;
+  export = (fun x -> match x with | Inl x -> Inl (c1.export x) | Inr x -> Inr (c2.export x));
+  lemma_export_preserves_prref = (fun x -> 
+    match x with | Inl x -> c1.lemma_export_preserves_prref x | Inr x -> c2.lemma_export_preserves_prref x)
+}
+
+instance exportable_pair t1 t2 {| c1:exportable_from t1 |} {| c2:exportable_from t2 |} : exportable_from (t1 * t2) = {
+  c_styp = witnessable_pair t1 t2 #c1.c_styp #c2.c_styp;
+  ityp = c1.ityp * c2.ityp;
+  c_ityp = targetlang_pair default_spec _ _ #c1.c_ityp #c2.c_ityp;
+  export = (fun (x1, x2) -> (c1.export x1, c2.export x2));
+  lemma_export_preserves_prref = (fun (x1, x2) -> c1.lemma_export_preserves_prref x1; c2.lemma_export_preserves_prref x2)
+}
 
 instance exportable_ref t {| c:targetlang default_spec t |} : exportable_from (ref t) = {
   c_styp = witnessable_mref t _ #c.wt;
@@ -56,29 +119,191 @@ instance exportable_arrow
   {| c2:exportable_from t2 |}
   (pre:(t1 -> st_pre))
   (post:(x:t1 -> h0:heap -> st_post' (resexn t2) (pre x h0)))
-  (_:squash (forall x h0 r h1. post x h0 r h1 ==>  post_targetlang_arrow default_spec #(resexn t2) #(witnessable_sum t2 unit #c2.c_styp) h0 r h1))
-  (check:(x:t1 -> ST bool All (fun h0 -> (Mktuple3?._1 default_spec) h0) (fun h0 r h1 -> h0==h1 /\ (r ==> pre x h0)))) 
+  (_:squash (forall x h0 r h1. post x h0 r h1 ==>  post_targetlang_arrow default_spec #(resexn t2) #(witnessable_sum t2 err #c2.c_styp) h0 r h1))
+  (check:(x:t1 -> ST (either unit err) All (fun h0 -> (Mktuple3?._1 default_spec) h0) (fun h0 r h1 -> h0==h1 /\ (Inl? r ==> pre x h0)))) 
                              (** ^ the fact that the check has a pre-condition means that the check does not have to enforce it
                                  e.g., the invariant on the heap **)
   : exportable_from (x:t1 -> ST (resexn t2) All (pre x) (post x)) = {
   c_styp = witnessable_arrow t1 (resexn t2) pre post;
-  ityp = mk_targetlang_arrow default_spec c1.ityp #c1.c_ityp.wt (resexn c2.ityp) #(witnessable_sum c2.ityp unit #c2.c_ityp.wt);
-  c_ityp = targetlang_arrow default_spec c1.ityp (resexn c2.ityp) #_ #(targetlang_sum default_spec c2.ityp unit) ;
+  ityp = mk_targetlang_arrow default_spec c1.ityp #c1.c_ityp.wt (resexn c2.ityp) #(witnessable_sum c2.ityp err #c2.c_ityp.wt);
+  c_ityp = targetlang_arrow default_spec c1.ityp (resexn c2.ityp) #_ #(targetlang_sum default_spec c2.ityp err) ;
   export = (fun (f:(x:t1 -> ST (resexn t2) All (pre x) (post x))) (x:c1.ityp) ->
     match c1.import x with
     | Inl x -> begin
-      if check x then begin
+      match check x with
+      | Inl _ -> begin
         match f x with
         | Inl r -> begin
           c2.lemma_export_preserves_prref r; (** the squash + this lemma imply the post-condition **)
           Inl (c2.export r)
         end
-        | Inr unit -> Inr unit
+        | Inr err -> Inr err
       end
-      else Inr ()
+      | Inr err -> Inr err
     end
-    | Inr () -> Inr ()
+    | Inr err -> Inr err
   );
   lemma_export_preserves_prref = (fun _  -> ());
 }
+
 (** Importable instances **)
+instance targetlang_is_safely_importable t {| c1:targetlang default_spec t |} : safe_importable_to t = {
+  c_styp = c1.wt;
+  ityp = t;
+  c_ityp = solve;
+  safe_import = (fun x -> x);
+  lemma_safe_import_preserves_prref = (fun _ -> ())
+}
+
+instance safe_importable_is_importable t {| c1:safe_importable_to t |} : importable_to t = {
+  c_styp = c1.c_styp;
+  ityp = c1.ityp;
+  c_ityp = c1.c_ityp;
+  import = (fun x -> Inl (c1.safe_import x));
+  lemma_import_preserves_prref = (fun x -> c1.lemma_safe_import_preserves_prref x);
+}
+
+instance safe_importable_unit : safe_importable_to unit = {
+  c_styp = witnessable_unit;
+  ityp = unit;
+  c_ityp = solve;
+  safe_import = (fun x -> x);
+  lemma_safe_import_preserves_prref = (fun _ -> ())
+}
+
+instance safe_importable_err : safe_importable_to err = {
+  c_styp = witnessable_err;
+  ityp = err;
+  c_ityp = solve;
+  safe_import = (fun x -> x);
+  lemma_safe_import_preserves_prref = (fun _ -> ())
+}
+
+instance importable_option t {| c:importable_to t |} : importable_to (option t) = {
+  c_styp = witnessable_option t #c.c_styp;
+  ityp = option c.ityp;
+  c_ityp = targetlang_option default_spec c.ityp #c.c_ityp;
+  import = (fun x -> 
+    match x with 
+    | Some x -> begin
+      match c.import x with
+      | Inl x -> Inl (Some x)
+      | Inr err -> Inr err
+    end 
+    | FStar.Pervasives.Native.None -> Inl FStar.Pervasives.Native.None);
+  lemma_import_preserves_prref = (fun x -> 
+    match x with 
+    | Some x -> c.lemma_import_preserves_prref x
+    | FStar.Pervasives.Native.None -> ())
+}
+
+instance importable_sum t1 t2 {| c1:importable_to t1 |} {| c2:importable_to t2 |} : importable_to (either t1 t2) = {
+  c_styp = witnessable_sum t1 t2 #c1.c_styp #c2.c_styp;
+  ityp = either c1.ityp c2.ityp;
+  c_ityp = targetlang_sum default_spec _ _ #c1.c_ityp #c2.c_ityp;
+  import = (fun x -> 
+    match x with 
+    | Inl x -> begin
+      match c1.import x with
+      | Inl x -> Inl (Inl x)
+      | Inr err -> Inr err
+    end 
+    | Inr x -> begin
+      match c2.import x with
+      | Inl x -> Inl (Inr x)
+      | Inr err -> Inr err
+    end);
+  lemma_import_preserves_prref = (fun x -> 
+    match x with 
+    | Inl x -> c1.lemma_import_preserves_prref x
+    | Inr x -> c2.lemma_import_preserves_prref x)
+}
+
+instance safe_importable_resexn t {| c:importable_to t |} : safe_importable_to (resexn t) = {
+  c_styp = witnessable_sum t err #c.c_styp;
+  ityp = resexn c.ityp;
+  c_ityp = targetlang_sum default_spec c.ityp err #c.c_ityp;
+  safe_import = (fun x ->
+    match x with
+    | Inl x -> begin
+      match c.import x with
+      | Inl x -> Inl x
+      | Inr err -> Inr err
+    end
+    | Inr err -> Inr err
+    );
+  lemma_safe_import_preserves_prref = (fun x ->
+    match x with
+    | Inl x -> c.lemma_import_preserves_prref x
+    | Inr err -> ())
+}
+
+type cb_capture_check (t1:Type) (t2:Type) {| c2: witnessable t2 |}
+  (pre:(t1 -> st_pre))
+  (post:(x:t1 -> h0:heap -> st_post' t2 (pre x h0)))
+  (x:t1)
+  (eh0:FStar.Ghost.erased heap{pre x eh0}) =
+  (r:t2 -> ST (resexn unit) All (fun h1 -> post_targetlang_arrow default_spec eh0 r h1) (fun h1 rck h1' -> 
+    h1 == h1' /\ (Inl? rck ==> post x eh0 r h1)))
+
+type capture_check
+  (t1:Type) (t2:Type) {| c2: witnessable t2 |}
+  (pre:(t1 -> st_pre))
+  (post:(x:t1 -> h0:heap -> st_post' t2 (pre x h0))) =
+  x:t1 -> ST (
+    eh0:FStar.Ghost.erased heap{pre x eh0} & cb_capture_check t1 t2 #c2 pre post x eh0
+  ) All (pre x) (fun h0 r h1 -> FStar.Ghost.reveal (dfst r) == h0 /\ h0 == h1)
+
+instance safe_importable_arrow 
+  (t1:Type) (t2:Type)
+  {| c1:exportable_from t1 |}
+  {| c2:importable_to t2 |}
+  (pre:(t1 -> st_pre))
+  (post:(x:t1 -> h0:heap -> st_post' (resexn t2) (pre x h0)))
+  (_:squash (forall (x:t1) h0. pre x h0 ==> pre_targetlang_arrow default_spec #_ #c1.c_styp x h0))
+  (_:squash (forall (x:t1) h0 r h1. pre x h0 /\ post_targetlang_arrow default_spec #_ #(witnessable_sum t2 err #c2.c_styp) h0 r h1 ==> 
+    (forall err. post x h0 (Inr err) h1)))
+  (capture_check:capture_check t1 (resexn t2) #(witnessable_sum _ err #c2.c_styp) pre post)
+  : safe_importable_to (x:t1 -> ST (resexn t2) All (pre x) (post x)) = {
+  c_styp = witnessable_arrow t1 (resexn t2) pre post;
+  ityp = mk_targetlang_arrow default_spec c1.ityp #c1.c_ityp.wt (resexn c2.ityp) #(witnessable_sum c2.ityp err #c2.c_ityp.wt);
+  c_ityp = targetlang_arrow default_spec c1.ityp (resexn c2.ityp) #_ #(targetlang_sum default_spec c2.ityp err #c2.c_ityp);
+  safe_import = (fun (f:mk_targetlang_arrow default_spec c1.ityp #c1.c_ityp.wt (resexn c2.ityp) #(witnessable_sum c2.ityp err #c2.c_ityp.wt)) (x:t1) ->
+    c1.lemma_export_preserves_prref x;
+    let (| _, check |) = capture_check x in
+    let x' = c1.export x in
+    let res : resexn c2.ityp = f x' in
+    let fres = (safe_importable_resexn t2).safe_import res in
+    (safe_importable_resexn t2).lemma_safe_import_preserves_prref res;
+    match check fres with
+    | Inl _ -> fres
+    | Inr err -> Inr err
+  );
+  lemma_safe_import_preserves_prref = (fun _ -> ())
+}
+
+type of_f = x:ref int -> SST (resexn unit) (requires (fun h0 -> satisfy x (Mktuple3?._2 default_spec))) (ensures (fun h0 r h1 -> Inr? r \/ sel h0 x == sel h1 x))
+
+let test : safe_importable_to of_f =
+  safe_importable_arrow 
+    (ref int) unit
+    (fun x -> sst_pre (fun h0 -> satisfy x (Mktuple3?._2 default_spec))) 
+    (fun x -> sst_post _ _ (fun h0 r h1 -> Inr? r \/ sel h0 x == sel h1 x)) 
+    ()
+    ()
+    (fun (rx:ref int) ->
+      recall (contains_pred rx);
+      let x = sst_read' rx in
+      let eh0 = get_heap () in
+      let check : cb_capture_check (ref int) (resexn unit) _ _ rx eh0 = 
+        (fun res -> if x = sst_read rx then Inl () else Inr (Contract_failure "x is not equal")) in
+      (| eh0, check |))
+
+val unsafe_f : mk_targetlang_arrow default_spec (ref int) (resexn unit)
+let unsafe_f x = 
+  recall (contains_pred x);
+  recall (is_shared x);
+  sst_write x 0;
+  Inl ()
+
+let safe_f = test.safe_import unsafe_f
